language/move-prover/bytecode-to-boogie/tests/goldenfiles/libra_account.bpl
@@ -61,7 +61,7 @@ function LibraCoin_T_type_value(): TypeValue {
 }
 procedure {:inline 1} Pack_LibraCoin_T(value: Value) returns (_struct: Value)
 {
-    assume IsValidInteger(value);
+    assume IsValidU64(value);
     _struct := Vector(ExtendValueArray(EmptyValueArray, value));
 
 }
@@ -70,7 +70,7 @@ procedure {:inline 1} Unpack_LibraCoin_T(_struct: Value) returns (value: Value)
 {
     assume is#Vector(_struct);
     value := SelectField(_struct, LibraCoin_T_value);
-    assume IsValidInteger(value);
+    assume IsValidU64(value);
 }
 
 const unique LibraCoin_MintCapability: TypeName;
@@ -101,7 +101,7 @@ function LibraCoin_MarketCap_type_value(): TypeValue {
 }
 procedure {:inline 1} Pack_LibraCoin_MarketCap(total_value: Value) returns (_struct: Value)
 {
-    assume IsValidInteger(total_value);
+    assume IsValidU64(total_value);
     _struct := Vector(ExtendValueArray(EmptyValueArray, total_value));
 
 }
@@ -110,7 +110,7 @@ procedure {:inline 1} Unpack_LibraCoin_MarketCap(_struct: Value) returns (total_
 {
     assume is#Vector(_struct);
     total_value := SelectField(_struct, LibraCoin_MarketCap_total_value);
-    assume IsValidInteger(total_value);
+    assume IsValidU64(total_value);
 }
 
 
@@ -138,7 +138,7 @@ ensures old(b#Boolean(Boolean(!(b#Boolean(ExistsResource(m, LibraCoin_MintCapabi
     saved_m := m;
 
     // assume arguments are of correct types
-    assume IsValidInteger(amount);
+    assume IsValidU64(amount);
 
     old_size := local_counter;
     local_counter := local_counter + 5;
@@ -214,7 +214,7 @@ ensures old(b#Boolean(Boolean(!(b#Boolean(ExistsResource(m, LibraCoin_MarketCap_
     saved_m := m;
 
     // assume arguments are of correct types
-    assume IsValidInteger(value);
+    assume IsValidU64(value);
     assume is#Vector(Dereference(m, capability));
     assume IsValidReferenceParameter(m, local_counter, capability);
 
@@ -236,7 +236,7 @@ ensures old(b#Boolean(Boolean(!(b#Boolean(ExistsResource(m, LibraCoin_MarketCap_
     call tmp := LdConst(1000000);
     m := UpdateLocal(m, old_size + 7, tmp);
 
-    call tmp := Mul(GetLocal(m, old_size + 6), GetLocal(m, old_size + 7));
+    call tmp := MulU64(GetLocal(m, old_size + 6), GetLocal(m, old_size + 7));
     if (abort_flag) { goto Label_Abort; }
     m := UpdateLocal(m, old_size + 8, tmp);
 
@@ -268,7 +268,7 @@ Label_11:
     call t15 := BorrowField(t14, LibraCoin_MarketCap_total_value);
 
     call tmp := ReadRef(t15);
-    assume IsValidInteger(tmp);
+    assume IsValidU64(tmp);
 
     m := UpdateLocal(m, old_size + 16, tmp);
 
@@ -281,7 +281,7 @@ Label_11:
     call tmp := CopyOrMoveValue(GetLocal(m, old_size + 0));
     m := UpdateLocal(m, old_size + 18, tmp);
 
-    call tmp := Add(GetLocal(m, old_size + 17), GetLocal(m, old_size + 18));
+    call tmp := AddU64(GetLocal(m, old_size + 17), GetLocal(m, old_size + 18));
     if (abort_flag) { goto Label_Abort; }
     m := UpdateLocal(m, old_size + 19, tmp);
 
@@ -430,7 +430,7 @@ ensures old(b#Boolean(Boolean(!(b#Boolean(ExistsResource(m, LibraCoin_MarketCap_
     call t2 := BorrowField(t1, LibraCoin_MarketCap_total_value);
 
     call tmp := ReadRef(t2);
-    assume IsValidInteger(tmp);
+    assume IsValidU64(tmp);
 
     m := UpdateLocal(m, old_size + 3, tmp);
 
@@ -520,7 +520,7 @@ ensures b#Boolean(Boolean((ret0) == (SelectField(Dereference(m, coin_ref), Libra
     call t2 := BorrowField(t1, LibraCoin_T_value);
 
     call tmp := ReadRef(t2);
-    assume IsValidInteger(tmp);
+    assume IsValidU64(tmp);
 
     m := UpdateLocal(m, old_size + 3, tmp);
 
@@ -562,7 +562,7 @@ ensures old(b#Boolean(Boolean(i#Integer(SelectField(coin, LibraCoin_T_value)) < 
 
     // assume arguments are of correct types
     assume is#Vector(coin);
-    assume IsValidInteger(amount);
+    assume IsValidU64(amount);
 
     old_size := local_counter;
     local_counter := local_counter + 8;
@@ -642,7 +642,7 @@ ensures old(b#Boolean(Boolean(i#Integer(SelectField(Dereference(m, coin_ref), Li
     // assume arguments are of correct types
     assume is#Vector(Dereference(m, coin_ref));
     assume IsValidReferenceParameter(m, local_counter, coin_ref);
-    assume IsValidInteger(amount);
+    assume IsValidU64(amount);
 
     old_size := local_counter;
     local_counter := local_counter + 18;
@@ -654,7 +654,7 @@ ensures old(b#Boolean(Boolean(i#Integer(SelectField(Dereference(m, coin_ref), Li
     call t4 := BorrowField(t3, LibraCoin_T_value);
 
     call tmp := ReadRef(t4);
-    assume IsValidInteger(tmp);
+    assume IsValidU64(tmp);
 
     m := UpdateLocal(m, old_size + 5, tmp);
 
@@ -815,7 +815,7 @@ ensures old(b#Boolean(Boolean(i#Integer(Integer(i#Integer(SelectField(Dereferenc
     call t5 := BorrowField(t4, LibraCoin_T_value);
 
     call tmp := ReadRef(t5);
-    assume IsValidInteger(tmp);
+    assume IsValidU64(tmp);
 
     m := UpdateLocal(m, old_size + 6, tmp);
 
@@ -837,7 +837,7 @@ ensures old(b#Boolean(Boolean(i#Integer(Integer(i#Integer(SelectField(Dereferenc
     call tmp := CopyOrMoveValue(GetLocal(m, old_size + 3));
     m := UpdateLocal(m, old_size + 10, tmp);
 
-    call tmp := Add(GetLocal(m, old_size + 9), GetLocal(m, old_size + 10));
+    call tmp := AddU64(GetLocal(m, old_size + 9), GetLocal(m, old_size + 10));
     if (abort_flag) { goto Label_Abort; }
     m := UpdateLocal(m, old_size + 11, tmp);
 
@@ -995,7 +995,7 @@ procedure {:inline 1} Pack_LibraAccount_T(authentication_key: Value, balance: Va
     assume is#Boolean(delegated_withdrawal_capability);
     assume is#Vector(received_events);
     assume is#Vector(sent_events);
-    assume IsValidInteger(sequence_number);
+    assume IsValidU64(sequence_number);
     assume is#Vector(event_generator);
     _struct := Vector(ExtendValueArray(ExtendValueArray(ExtendValueArray(ExtendValueArray(ExtendValueArray(ExtendValueArray(ExtendValueArray(ExtendValueArray(EmptyValueArray, authentication_key), balance), delegated_key_rotation_capability), delegated_withdrawal_capability), received_events), sent_events), sequence_number), event_generator));
 
@@ -1017,7 +1017,7 @@ procedure {:inline 1} Unpack_LibraAccount_T(_struct: Value) returns (authenticat
     sent_events := SelectField(_struct, LibraAccount_T_sent_events);
     assume is#Vector(sent_events);
     sequence_number := SelectField(_struct, LibraAccount_T_sequence_number);
-    assume IsValidInteger(sequence_number);
+    assume IsValidU64(sequence_number);
     event_generator := SelectField(_struct, LibraAccount_T_event_generator);
     assume is#Vector(event_generator);
 }
@@ -1074,7 +1074,7 @@ function LibraAccount_SentPaymentEvent_type_value(): TypeValue {
 }
 procedure {:inline 1} Pack_LibraAccount_SentPaymentEvent(amount: Value, payee: Value, metadata: Value) returns (_struct: Value)
 {
-    assume IsValidInteger(amount);
+    assume IsValidU64(amount);
     assume is#Address(payee);
     assume is#ByteArray(metadata);
     _struct := Vector(ExtendValueArray(ExtendValueArray(ExtendValueArray(EmptyValueArray, amount), payee), metadata));
@@ -1085,7 +1085,7 @@ procedure {:inline 1} Unpack_LibraAccount_SentPaymentEvent(_struct: Value) retur
 {
     assume is#Vector(_struct);
     amount := SelectField(_struct, LibraAccount_SentPaymentEvent_amount);
-    assume IsValidInteger(amount);
+    assume IsValidU64(amount);
     payee := SelectField(_struct, LibraAccount_SentPaymentEvent_payee);
     assume is#Address(payee);
     metadata := SelectField(_struct, LibraAccount_SentPaymentEvent_metadata);
@@ -1104,7 +1104,7 @@ function LibraAccount_ReceivedPaymentEvent_type_value(): TypeValue {
 }
 procedure {:inline 1} Pack_LibraAccount_ReceivedPaymentEvent(amount: Value, payer: Value, metadata: Value) returns (_struct: Value)
 {
-    assume IsValidInteger(amount);
+    assume IsValidU64(amount);
     assume is#Address(payer);
     assume is#ByteArray(metadata);
     _struct := Vector(ExtendValueArray(ExtendValueArray(ExtendValueArray(EmptyValueArray, amount), payer), metadata));
@@ -1115,7 +1115,7 @@ procedure {:inline 1} Unpack_LibraAccount_ReceivedPaymentEvent(_struct: Value) r
 {
     assume is#Vector(_struct);
     amount := SelectField(_struct, LibraAccount_ReceivedPaymentEvent_amount);
-    assume IsValidInteger(amount);
+    assume IsValidU64(amount);
     payer := SelectField(_struct, LibraAccount_ReceivedPaymentEvent_payer);
     assume is#Address(payer);
     metadata := SelectField(_struct, LibraAccount_ReceivedPaymentEvent_metadata);
@@ -1130,7 +1130,7 @@ function LibraAccount_EventHandleGenerator_type_value(): TypeValue {
 }
 procedure {:inline 1} Pack_LibraAccount_EventHandleGenerator(counter: Value) returns (_struct: Value)
 {
-    assume IsValidInteger(counter);
+    assume IsValidU64(counter);
     _struct := Vector(ExtendValueArray(EmptyValueArray, counter));
 
 }
@@ -1139,7 +1139,7 @@ procedure {:inline 1} Unpack_LibraAccount_EventHandleGenerator(_struct: Value) r
 {
     assume is#Vector(_struct);
     counter := SelectField(_struct, LibraAccount_EventHandleGenerator_counter);
-    assume IsValidInteger(counter);
+    assume IsValidU64(counter);
 }
 
 const unique LibraAccount_EventHandle: TypeName;
@@ -1152,7 +1152,7 @@ function LibraAccount_EventHandle_type_value(tv0: TypeValue): TypeValue {
 }
 procedure {:inline 1} Pack_LibraAccount_EventHandle(tv0: TypeValue, counter: Value, guid: Value) returns (_struct: Value)
 {
-    assume IsValidInteger(counter);
+    assume IsValidU64(counter);
     assume is#ByteArray(guid);
     _struct := Vector(ExtendValueArray(ExtendValueArray(EmptyValueArray, counter), guid));
 
@@ -1162,7 +1162,7 @@ procedure {:inline 1} Unpack_LibraAccount_EventHandle(_struct: Value) returns (c
 {
     assume is#Vector(_struct);
     counter := SelectField(_struct, LibraAccount_EventHandle_counter);
-    assume IsValidInteger(counter);
+    assume IsValidU64(counter);
     guid := SelectField(_struct, LibraAccount_EventHandle_guid);
     assume is#ByteArray(guid);
 }
@@ -1489,7 +1489,7 @@ ensures old(b#Boolean(Boolean(!(b#Boolean(ExistsResource(m, LibraAccount_T_type_
 
     call t8 := LibraCoin_value(t7);
     if (abort_flag) { goto Label_Abort; }
-    assume IsValidInteger(t8);
+    assume IsValidU64(t8);
 
     m := UpdateLocal(m, old_size + 8, t8);
 
@@ -1615,7 +1615,7 @@ requires ExistsTxnSenderAccount(m, txn);
 
     // assume arguments are of correct types
     assume is#Address(payee);
-    assume IsValidInteger(amount);
+    assume IsValidU64(amount);
 
     old_size := local_counter;
     local_counter := local_counter + 9;
@@ -1695,7 +1695,7 @@ ensures old(b#Boolean(Boolean(i#Integer(SelectField(SelectField(Dereference(m, a
     // assume arguments are of correct types
     assume is#Vector(Dereference(m, account));
     assume IsValidReferenceParameter(m, local_counter, account);
-    assume IsValidInteger(amount);
+    assume IsValidU64(amount);
 
     old_size := local_counter;
     local_counter := local_counter + 8;
@@ -1763,7 +1763,7 @@ ensures old(b#Boolean(SelectField(Dereference(m, GetResourceReference(LibraAccou
     saved_m := m;
 
     // assume arguments are of correct types
-    assume IsValidInteger(amount);
+    assume IsValidU64(amount);
 
     old_size := local_counter;
     local_counter := local_counter + 11;
@@ -1849,7 +1849,7 @@ ensures old(b#Boolean(Boolean(!(b#Boolean(ExistsResource(m, LibraAccount_T_type_
     // assume arguments are of correct types
     assume is#Vector(Dereference(m, cap));
     assume IsValidReferenceParameter(m, local_counter, cap);
-    assume IsValidInteger(amount);
+    assume IsValidU64(amount);
 
     old_size := local_counter;
     local_counter := local_counter + 10;
@@ -2096,7 +2096,7 @@ requires ExistsTxnSenderAccount(m, txn);
     assume is#Address(payee);
     assume is#Vector(Dereference(m, cap));
     assume IsValidReferenceParameter(m, local_counter, cap);
-    assume IsValidInteger(amount);
+    assume IsValidU64(amount);
     assume is#ByteArray(metadata);
 
     old_size := local_counter;
@@ -2198,7 +2198,7 @@ ensures old(b#Boolean(SelectField(Dereference(m, GetResourceReference(LibraAccou
 
     // assume arguments are of correct types
     assume is#Address(payee);
-    assume IsValidInteger(amount);
+    assume IsValidU64(amount);
     assume is#ByteArray(metadata);
 
     old_size := local_counter;
@@ -2306,7 +2306,7 @@ ensures old(b#Boolean(SelectField(Dereference(m, GetResourceReference(LibraAccou
 
     // assume arguments are of correct types
     assume is#Address(payee);
-    assume IsValidInteger(amount);
+    assume IsValidU64(amount);
 
     old_size := local_counter;
     local_counter := local_counter + 10;
@@ -2860,7 +2860,7 @@ ensures old(b#Boolean(ExistsResource(m, LibraAccount_T_type_value(), a#Address(f
 
     // assume arguments are of correct types
     assume is#Address(fresh_address);
-    assume IsValidInteger(initial_balance);
+    assume IsValidU64(initial_balance);
 
     old_size := local_counter;
     local_counter := local_counter + 8;
@@ -2941,7 +2941,7 @@ ensures b#Boolean(Boolean((ret0) == (SelectField(SelectField(Dereference(m, acco
 
     call t4 := LibraCoin_value(t3);
     if (abort_flag) { goto Label_Abort; }
-    assume IsValidInteger(t4);
+    assume IsValidU64(t4);
 
     m := UpdateLocal(m, old_size + 4, t4);
 
@@ -3000,7 +3000,7 @@ ensures old(b#Boolean(Boolean(!(b#Boolean(ExistsResource(m, LibraAccount_T_type_
 
     call t3 := LibraAccount_balance_for_account(t2);
     if (abort_flag) { goto Label_Abort; }
-    assume IsValidInteger(t3);
+    assume IsValidU64(t3);
 
     m := UpdateLocal(m, old_size + 3, t3);
 
@@ -3048,7 +3048,7 @@ ensures b#Boolean(Boolean((ret0) == (SelectField(Dereference(m, account), LibraA
     call t2 := BorrowField(t1, LibraAccount_T_sequence_number);
 
     call tmp := ReadRef(t2);
-    assume IsValidInteger(tmp);
+    assume IsValidU64(tmp);
 
     m := UpdateLocal(m, old_size + 3, tmp);
 
@@ -3101,7 +3101,7 @@ ensures old(b#Boolean(Boolean(!(b#Boolean(ExistsResource(m, LibraAccount_T_type_
 
     call t3 := LibraAccount_sequence_number_for_account(t2);
     if (abort_flag) { goto Label_Abort; }
-    assume IsValidInteger(t3);
+    assume IsValidU64(t3);
 
     m := UpdateLocal(m, old_size + 3, t3);
 
@@ -3415,10 +3415,10 @@ requires ExistsTxnSenderAccount(m, txn);
     saved_m := m;
 
     // assume arguments are of correct types
-    assume IsValidInteger(txn_sequence_number);
+    assume IsValidU64(txn_sequence_number);
     assume is#ByteArray(txn_public_key);
-    assume IsValidInteger(txn_gas_price);
-    assume IsValidInteger(txn_max_gas_units);
+    assume IsValidU64(txn_gas_price);
+    assume IsValidU64(txn_max_gas_units);
 
     old_size := local_counter;
     local_counter := local_counter + 50;
@@ -3499,7 +3499,7 @@ Label_21:
     call tmp := CopyOrMoveValue(GetLocal(m, old_size + 3));
     m := UpdateLocal(m, old_size + 26, tmp);
 
-    call tmp := Mul(GetLocal(m, old_size + 25), GetLocal(m, old_size + 26));
+    call tmp := MulU64(GetLocal(m, old_size + 25), GetLocal(m, old_size + 26));
     if (abort_flag) { goto Label_Abort; }
     m := UpdateLocal(m, old_size + 27, tmp);
 
@@ -3516,7 +3516,7 @@ Label_21:
 
     call t31 := LibraAccount_balance_for_account(t30);
     if (abort_flag) { goto Label_Abort; }
-    assume IsValidInteger(t31);
+    assume IsValidU64(t31);
 
     m := UpdateLocal(m, old_size + 31, t31);
 
@@ -3549,7 +3549,7 @@ Label_38:
     call t38 := BorrowField(t37, LibraAccount_T_sequence_number);
 
     call tmp := ReadRef(t38);
-    assume IsValidInteger(tmp);
+    assume IsValidU64(tmp);
 
     m := UpdateLocal(m, old_size + 39, tmp);
 
@@ -3657,10 +3657,10 @@ requires ExistsTxnSenderAccount(m, txn);
     saved_m := m;
 
     // assume arguments are of correct types
-    assume IsValidInteger(txn_sequence_number);
-    assume IsValidInteger(txn_gas_price);
-    assume IsValidInteger(txn_max_gas_units);
-    assume IsValidInteger(gas_units_remaining);
+    assume IsValidU64(txn_sequence_number);
+    assume IsValidU64(txn_gas_price);
+    assume IsValidU64(txn_max_gas_units);
+    assume IsValidU64(gas_units_remaining);
 
     old_size := local_counter;
     local_counter := local_counter + 37;
@@ -3691,7 +3691,7 @@ requires ExistsTxnSenderAccount(m, txn);
     if (abort_flag) { goto Label_Abort; }
     m := UpdateLocal(m, old_size + 14, tmp);
 
-    call tmp := Mul(GetLocal(m, old_size + 11), GetLocal(m, old_size + 14));
+    call tmp := MulU64(GetLocal(m, old_size + 11), GetLocal(m, old_size + 14));
     if (abort_flag) { goto Label_Abort; }
     m := UpdateLocal(m, old_size + 15, tmp);
 
@@ -3708,7 +3708,7 @@ requires ExistsTxnSenderAccount(m, txn);
 
     call t19 := LibraAccount_balance_for_account(t18);
     if (abort_flag) { goto Label_Abort; }
-    assume IsValidInteger(t19);
+    assume IsValidU64(t19);
 
     m := UpdateLocal(m, old_size + 19, t19);
 
@@ -3750,7 +3750,7 @@ Label_20:
     call tmp := LdConst(1);
     m := UpdateLocal(m, old_size + 28, tmp);
 
-    call tmp := Add(GetLocal(m, old_size + 27), GetLocal(m, old_size + 28));
+    call tmp := AddU64(GetLocal(m, old_size + 27), GetLocal(m, old_size + 28));
     if (abort_flag) { goto Label_Abort; }
     m := UpdateLocal(m, old_size + 29, tmp);
 
@@ -3853,7 +3853,7 @@ ensures old(b#Boolean(Boolean(true))) ==> !abort_flag;
     call t10 := CopyOrMoveRef(t2);
 
     call tmp := ReadRef(t10);
-    assume IsValidInteger(tmp);
+    assume IsValidU64(tmp);
 
     m := UpdateLocal(m, old_size + 11, tmp);
 
@@ -3869,7 +3869,7 @@ ensures old(b#Boolean(Boolean(true))) ==> !abort_flag;
     call t13 := CopyOrMoveRef(t2);
 
     call tmp := ReadRef(t13);
-    assume IsValidInteger(tmp);
+    assume IsValidU64(tmp);
 
     m := UpdateLocal(m, old_size + 14, tmp);
 
@@ -4093,7 +4093,7 @@ ensures old(b#Boolean(Boolean(true))) ==> !abort_flag;
     call t10 := CopyOrMoveRef(t2);
 
     call tmp := ReadRef(t10);
-    assume IsValidInteger(tmp);
+    assume IsValidU64(tmp);
 
     m := UpdateLocal(m, old_size + 11, tmp);
 
@@ -4106,7 +4106,7 @@ ensures old(b#Boolean(Boolean(true))) ==> !abort_flag;
     call t13 := CopyOrMoveRef(t2);
 
     call tmp := ReadRef(t13);
-    assume IsValidInteger(tmp);
+    assume IsValidU64(tmp);
 
     m := UpdateLocal(m, old_size + 14, tmp);
 
