language/move-prover/bytecode-to-boogie/tests/goldenfiles/test-access-path.bpl
@@ -57,7 +57,7 @@ function LibraCoin_T_type_value(): TypeValue {
 }
 procedure {:inline 1} Pack_LibraCoin_T(value: Value) returns (_struct: Value)
 {
-    assume IsValidInteger(value);
+    assume IsValidU64(value);
     _struct := Vector(ExtendValueArray(EmptyValueArray, value));
 
 }
@@ -66,7 +66,7 @@ procedure {:inline 1} Unpack_LibraCoin_T(_struct: Value) returns (value: Value)
 {
     assume is#Vector(_struct);
     value := SelectField(_struct, LibraCoin_T_value);
-    assume IsValidInteger(value);
+    assume IsValidU64(value);
 }
 
 const unique LibraCoin_MintCapability: TypeName;
@@ -97,7 +97,7 @@ function LibraCoin_MarketCap_type_value(): TypeValue {
 }
 procedure {:inline 1} Pack_LibraCoin_MarketCap(total_value: Value) returns (_struct: Value)
 {
-    assume IsValidInteger(total_value);
+    assume IsValidU128(total_value);
     _struct := Vector(ExtendValueArray(EmptyValueArray, total_value));
 
 }
@@ -106,7 +106,7 @@ procedure {:inline 1} Unpack_LibraCoin_MarketCap(_struct: Value) returns (total_
 {
     assume is#Vector(_struct);
     total_value := SelectField(_struct, LibraCoin_MarketCap_total_value);
-    assume IsValidInteger(total_value);
+    assume IsValidU128(total_value);
 }
 
 
@@ -130,7 +130,7 @@ requires ExistsTxnSenderAccount(m, txn);
     saved_m := m;
 
     // assume arguments are of correct types
-    assume IsValidInteger(amount);
+    assume IsValidU64(amount);
 
     old_size := local_counter;
     local_counter := local_counter + 5;
@@ -199,7 +199,7 @@ requires ExistsTxnSenderAccount(m, txn);
     saved_m := m;
 
     // assume arguments are of correct types
-    assume IsValidInteger(value);
+    assume IsValidU64(value);
     assume is#Vector(Dereference(m, capability));
     assume IsValidReferenceParameter(m, local_counter, capability);
 
@@ -217,7 +217,7 @@ requires ExistsTxnSenderAccount(m, txn);
     call tmp := LdConst(1000000);
     m := UpdateLocal(m, old_size + 5, tmp);
 
-    call tmp := Mul(GetLocal(m, old_size + 4), GetLocal(m, old_size + 5));
+    call tmp := MulU64(GetLocal(m, old_size + 4), GetLocal(m, old_size + 5));
     if (abort_flag) { goto Label_Abort; }
     m := UpdateLocal(m, old_size + 6, tmp);
 
@@ -249,16 +249,18 @@ Label_9:
     call t13 := CopyOrMoveRef(t2);
 
     call tmp := ReadRef(t13);
-    assume IsValidInteger(tmp);
+    assume IsValidU128(tmp);
 
     m := UpdateLocal(m, old_size + 14, tmp);
 
     call tmp := CopyOrMoveValue(GetLocal(m, old_size + 0));
     m := UpdateLocal(m, old_size + 15, tmp);
 
-    m := UpdateLocal(m, old_size + 16, GetLocal(m, old_size + 15));
+    call tmp := CastU128(GetLocal(m, old_size + 15));
+    if (abort_flag) { goto Label_Abort; }
+    m := UpdateLocal(m, old_size + 16, tmp);
 
-    call tmp := Add(GetLocal(m, old_size + 14), GetLocal(m, old_size + 16));
+    call tmp := AddU128(GetLocal(m, old_size + 14), GetLocal(m, old_size + 16));
     if (abort_flag) { goto Label_Abort; }
     m := UpdateLocal(m, old_size + 17, tmp);
 
@@ -397,7 +399,7 @@ requires ExistsTxnSenderAccount(m, txn);
     call t2 := BorrowField(t1, LibraCoin_MarketCap_total_value);
 
     call tmp := ReadRef(t2);
-    assume IsValidInteger(tmp);
+    assume IsValidU128(tmp);
 
     m := UpdateLocal(m, old_size + 3, tmp);
 
@@ -485,7 +487,7 @@ requires ExistsTxnSenderAccount(m, txn);
     call t2 := BorrowField(t1, LibraCoin_T_value);
 
     call tmp := ReadRef(t2);
-    assume IsValidInteger(tmp);
+    assume IsValidU64(tmp);
 
     m := UpdateLocal(m, old_size + 3, tmp);
 
@@ -524,7 +526,7 @@ requires ExistsTxnSenderAccount(m, txn);
 
     // assume arguments are of correct types
     assume is#Vector(coin);
-    assume IsValidInteger(amount);
+    assume IsValidU64(amount);
 
     old_size := local_counter;
     local_counter := local_counter + 8;
@@ -600,7 +602,7 @@ requires ExistsTxnSenderAccount(m, txn);
     // assume arguments are of correct types
     assume is#Vector(Dereference(m, coin_ref));
     assume IsValidReferenceParameter(m, local_counter, coin_ref);
-    assume IsValidInteger(amount);
+    assume IsValidU64(amount);
 
     old_size := local_counter;
     local_counter := local_counter + 18;
@@ -612,7 +614,7 @@ requires ExistsTxnSenderAccount(m, txn);
     call t4 := BorrowField(t3, LibraCoin_T_value);
 
     call tmp := ReadRef(t4);
-    assume IsValidInteger(tmp);
+    assume IsValidU64(tmp);
 
     m := UpdateLocal(m, old_size + 5, tmp);
 
@@ -767,7 +769,7 @@ requires ExistsTxnSenderAccount(m, txn);
     call t5 := BorrowField(t4, LibraCoin_T_value);
 
     call tmp := ReadRef(t5);
-    assume IsValidInteger(tmp);
+    assume IsValidU64(tmp);
 
     m := UpdateLocal(m, old_size + 6, tmp);
 
@@ -789,7 +791,7 @@ requires ExistsTxnSenderAccount(m, txn);
     call tmp := CopyOrMoveValue(GetLocal(m, old_size + 3));
     m := UpdateLocal(m, old_size + 10, tmp);
 
-    call tmp := Add(GetLocal(m, old_size + 9), GetLocal(m, old_size + 10));
+    call tmp := AddU64(GetLocal(m, old_size + 9), GetLocal(m, old_size + 10));
     if (abort_flag) { goto Label_Abort; }
     m := UpdateLocal(m, old_size + 11, tmp);
 
@@ -913,7 +915,7 @@ procedure {:inline 1} Pack_LibraAccount_T(authentication_key: Value, balance: Va
     assume is#Boolean(delegated_withdrawal_capability);
     assume is#Vector(received_events);
     assume is#Vector(sent_events);
-    assume IsValidInteger(sequence_number);
+    assume IsValidU64(sequence_number);
     assume is#Vector(event_generator);
     _struct := Vector(ExtendValueArray(ExtendValueArray(ExtendValueArray(ExtendValueArray(ExtendValueArray(ExtendValueArray(ExtendValueArray(ExtendValueArray(EmptyValueArray, authentication_key), balance), delegated_key_rotation_capability), delegated_withdrawal_capability), received_events), sent_events), sequence_number), event_generator));
 
@@ -935,7 +937,7 @@ procedure {:inline 1} Unpack_LibraAccount_T(_struct: Value) returns (authenticat
     sent_events := SelectField(_struct, LibraAccount_T_sent_events);
     assume is#Vector(sent_events);
     sequence_number := SelectField(_struct, LibraAccount_T_sequence_number);
-    assume IsValidInteger(sequence_number);
+    assume IsValidU64(sequence_number);
     event_generator := SelectField(_struct, LibraAccount_T_event_generator);
     assume is#Vector(event_generator);
 }
@@ -992,7 +994,7 @@ function LibraAccount_SentPaymentEvent_type_value(): TypeValue {
 }
 procedure {:inline 1} Pack_LibraAccount_SentPaymentEvent(amount: Value, payee: Value, metadata: Value) returns (_struct: Value)
 {
-    assume IsValidInteger(amount);
+    assume IsValidU64(amount);
     assume is#Address(payee);
     assume is#ByteArray(metadata);
     _struct := Vector(ExtendValueArray(ExtendValueArray(ExtendValueArray(EmptyValueArray, amount), payee), metadata));
@@ -1003,7 +1005,7 @@ procedure {:inline 1} Unpack_LibraAccount_SentPaymentEvent(_struct: Value) retur
 {
     assume is#Vector(_struct);
     amount := SelectField(_struct, LibraAccount_SentPaymentEvent_amount);
-    assume IsValidInteger(amount);
+    assume IsValidU64(amount);
     payee := SelectField(_struct, LibraAccount_SentPaymentEvent_payee);
     assume is#Address(payee);
     metadata := SelectField(_struct, LibraAccount_SentPaymentEvent_metadata);
@@ -1022,7 +1024,7 @@ function LibraAccount_ReceivedPaymentEvent_type_value(): TypeValue {
 }
 procedure {:inline 1} Pack_LibraAccount_ReceivedPaymentEvent(amount: Value, payer: Value, metadata: Value) returns (_struct: Value)
 {
-    assume IsValidInteger(amount);
+    assume IsValidU64(amount);
     assume is#Address(payer);
     assume is#ByteArray(metadata);
     _struct := Vector(ExtendValueArray(ExtendValueArray(ExtendValueArray(EmptyValueArray, amount), payer), metadata));
@@ -1033,7 +1035,7 @@ procedure {:inline 1} Unpack_LibraAccount_ReceivedPaymentEvent(_struct: Value) r
 {
     assume is#Vector(_struct);
     amount := SelectField(_struct, LibraAccount_ReceivedPaymentEvent_amount);
-    assume IsValidInteger(amount);
+    assume IsValidU64(amount);
     payer := SelectField(_struct, LibraAccount_ReceivedPaymentEvent_payer);
     assume is#Address(payer);
     metadata := SelectField(_struct, LibraAccount_ReceivedPaymentEvent_metadata);
@@ -1048,7 +1050,7 @@ function LibraAccount_EventHandleGenerator_type_value(): TypeValue {
 }
 procedure {:inline 1} Pack_LibraAccount_EventHandleGenerator(counter: Value) returns (_struct: Value)
 {
-    assume IsValidInteger(counter);
+    assume IsValidU64(counter);
     _struct := Vector(ExtendValueArray(EmptyValueArray, counter));
 
 }
@@ -1057,7 +1059,7 @@ procedure {:inline 1} Unpack_LibraAccount_EventHandleGenerator(_struct: Value) r
 {
     assume is#Vector(_struct);
     counter := SelectField(_struct, LibraAccount_EventHandleGenerator_counter);
-    assume IsValidInteger(counter);
+    assume IsValidU64(counter);
 }
 
 const unique LibraAccount_EventHandle: TypeName;
@@ -1070,7 +1072,7 @@ function LibraAccount_EventHandle_type_value(tv0: TypeValue): TypeValue {
 }
 procedure {:inline 1} Pack_LibraAccount_EventHandle(tv0: TypeValue, counter: Value, guid: Value) returns (_struct: Value)
 {
-    assume IsValidInteger(counter);
+    assume IsValidU64(counter);
     assume is#ByteArray(guid);
     _struct := Vector(ExtendValueArray(ExtendValueArray(EmptyValueArray, counter), guid));
 
@@ -1080,7 +1082,7 @@ procedure {:inline 1} Unpack_LibraAccount_EventHandle(_struct: Value) returns (c
 {
     assume is#Vector(_struct);
     counter := SelectField(_struct, LibraAccount_EventHandle_counter);
-    assume IsValidInteger(counter);
+    assume IsValidU64(counter);
     guid := SelectField(_struct, LibraAccount_EventHandle_guid);
     assume is#ByteArray(guid);
 }
@@ -1253,7 +1255,7 @@ requires ExistsTxnSenderAccount(m, txn);
 
     call t8 := LibraCoin_value(t7);
     if (abort_flag) { goto Label_Abort; }
-    assume IsValidInteger(t8);
+    assume IsValidU64(t8);
 
     m := UpdateLocal(m, old_size + 8, t8);
 
@@ -1379,7 +1381,7 @@ requires ExistsTxnSenderAccount(m, txn);
 
     // assume arguments are of correct types
     assume is#Address(payee);
-    assume IsValidInteger(amount);
+    assume IsValidU64(amount);
 
     old_size := local_counter;
     local_counter := local_counter + 9;
@@ -1455,7 +1457,7 @@ requires ExistsTxnSenderAccount(m, txn);
     // assume arguments are of correct types
     assume is#Vector(Dereference(m, account));
     assume IsValidReferenceParameter(m, local_counter, account);
-    assume IsValidInteger(amount);
+    assume IsValidU64(amount);
 
     old_size := local_counter;
     local_counter := local_counter + 8;
@@ -1519,7 +1521,7 @@ requires ExistsTxnSenderAccount(m, txn);
     saved_m := m;
 
     // assume arguments are of correct types
-    assume IsValidInteger(amount);
+    assume IsValidU64(amount);
 
     old_size := local_counter;
     local_counter := local_counter + 11;
@@ -1601,7 +1603,7 @@ requires ExistsTxnSenderAccount(m, txn);
     // assume arguments are of correct types
     assume is#Vector(Dereference(m, cap));
     assume IsValidReferenceParameter(m, local_counter, cap);
-    assume IsValidInteger(amount);
+    assume IsValidU64(amount);
 
     old_size := local_counter;
     local_counter := local_counter + 10;
@@ -1841,7 +1843,7 @@ requires ExistsTxnSenderAccount(m, txn);
     assume is#Address(payee);
     assume is#Vector(Dereference(m, cap));
     assume IsValidReferenceParameter(m, local_counter, cap);
-    assume IsValidInteger(amount);
+    assume IsValidU64(amount);
     assume is#ByteArray(metadata);
 
     old_size := local_counter;
@@ -1934,7 +1936,7 @@ requires ExistsTxnSenderAccount(m, txn);
 
     // assume arguments are of correct types
     assume is#Address(payee);
-    assume IsValidInteger(amount);
+    assume IsValidU64(amount);
     assume is#ByteArray(metadata);
 
     old_size := local_counter;
@@ -2011,7 +2013,7 @@ requires ExistsTxnSenderAccount(m, txn);
 
     // assume arguments are of correct types
     assume is#Address(payee);
-    assume IsValidInteger(amount);
+    assume IsValidU64(amount);
 
     old_size := local_counter;
     local_counter := local_counter + 5;
@@ -2521,7 +2523,7 @@ requires ExistsTxnSenderAccount(m, txn);
 
     // assume arguments are of correct types
     assume is#Address(fresh_address);
-    assume IsValidInteger(initial_balance);
+    assume IsValidU64(initial_balance);
 
     old_size := local_counter;
     local_counter := local_counter + 8;
@@ -2604,7 +2606,7 @@ requires ExistsTxnSenderAccount(m, txn);
 
     call t4 := LibraCoin_value(t3);
     if (abort_flag) { goto Label_Abort; }
-    assume IsValidInteger(t4);
+    assume IsValidU64(t4);
 
     m := UpdateLocal(m, old_size + 4, t4);
 
@@ -2660,7 +2662,7 @@ requires ExistsTxnSenderAccount(m, txn);
 
     call t3 := LibraAccount_balance_for_account(t2);
     if (abort_flag) { goto Label_Abort; }
-    assume IsValidInteger(t3);
+    assume IsValidU64(t3);
 
     m := UpdateLocal(m, old_size + 3, t3);
 
@@ -2707,7 +2709,7 @@ requires ExistsTxnSenderAccount(m, txn);
     call t2 := BorrowField(t1, LibraAccount_T_sequence_number);
 
     call tmp := ReadRef(t2);
-    assume IsValidInteger(tmp);
+    assume IsValidU64(tmp);
 
     m := UpdateLocal(m, old_size + 3, tmp);
 
@@ -2757,7 +2759,7 @@ requires ExistsTxnSenderAccount(m, txn);
 
     call t3 := LibraAccount_sequence_number_for_account(t2);
     if (abort_flag) { goto Label_Abort; }
-    assume IsValidInteger(t3);
+    assume IsValidU64(t3);
 
     m := UpdateLocal(m, old_size + 3, t3);
 
@@ -3064,10 +3066,10 @@ requires ExistsTxnSenderAccount(m, txn);
     saved_m := m;
 
     // assume arguments are of correct types
-    assume IsValidInteger(txn_sequence_number);
+    assume IsValidU64(txn_sequence_number);
     assume is#ByteArray(txn_public_key);
-    assume IsValidInteger(txn_gas_price);
-    assume IsValidInteger(txn_max_gas_units);
+    assume IsValidU64(txn_gas_price);
+    assume IsValidU64(txn_max_gas_units);
 
     old_size := local_counter;
     local_counter := local_counter + 50;
@@ -3148,7 +3150,7 @@ Label_21:
     call tmp := CopyOrMoveValue(GetLocal(m, old_size + 3));
     m := UpdateLocal(m, old_size + 26, tmp);
 
-    call tmp := Mul(GetLocal(m, old_size + 25), GetLocal(m, old_size + 26));
+    call tmp := MulU64(GetLocal(m, old_size + 25), GetLocal(m, old_size + 26));
     if (abort_flag) { goto Label_Abort; }
     m := UpdateLocal(m, old_size + 27, tmp);
 
@@ -3165,7 +3167,7 @@ Label_21:
 
     call t31 := LibraAccount_balance_for_account(t30);
     if (abort_flag) { goto Label_Abort; }
-    assume IsValidInteger(t31);
+    assume IsValidU64(t31);
 
     m := UpdateLocal(m, old_size + 31, t31);
 
@@ -3198,7 +3200,7 @@ Label_38:
     call t38 := BorrowField(t37, LibraAccount_T_sequence_number);
 
     call tmp := ReadRef(t38);
-    assume IsValidInteger(tmp);
+    assume IsValidU64(tmp);
 
     m := UpdateLocal(m, old_size + 39, tmp);
 
@@ -3306,10 +3308,10 @@ requires ExistsTxnSenderAccount(m, txn);
     saved_m := m;
 
     // assume arguments are of correct types
-    assume IsValidInteger(txn_sequence_number);
-    assume IsValidInteger(txn_gas_price);
-    assume IsValidInteger(txn_max_gas_units);
-    assume IsValidInteger(gas_units_remaining);
+    assume IsValidU64(txn_sequence_number);
+    assume IsValidU64(txn_gas_price);
+    assume IsValidU64(txn_max_gas_units);
+    assume IsValidU64(gas_units_remaining);
 
     old_size := local_counter;
     local_counter := local_counter + 37;
@@ -3340,7 +3342,7 @@ requires ExistsTxnSenderAccount(m, txn);
     if (abort_flag) { goto Label_Abort; }
     m := UpdateLocal(m, old_size + 14, tmp);
 
-    call tmp := Mul(GetLocal(m, old_size + 11), GetLocal(m, old_size + 14));
+    call tmp := MulU64(GetLocal(m, old_size + 11), GetLocal(m, old_size + 14));
     if (abort_flag) { goto Label_Abort; }
     m := UpdateLocal(m, old_size + 15, tmp);
 
@@ -3357,7 +3359,7 @@ requires ExistsTxnSenderAccount(m, txn);
 
     call t19 := LibraAccount_balance_for_account(t18);
     if (abort_flag) { goto Label_Abort; }
-    assume IsValidInteger(t19);
+    assume IsValidU64(t19);
 
     m := UpdateLocal(m, old_size + 19, t19);
 
@@ -3399,7 +3401,7 @@ Label_20:
     call tmp := LdConst(1);
     m := UpdateLocal(m, old_size + 28, tmp);
 
-    call tmp := Add(GetLocal(m, old_size + 27), GetLocal(m, old_size + 28));
+    call tmp := AddU64(GetLocal(m, old_size + 27), GetLocal(m, old_size + 28));
     if (abort_flag) { goto Label_Abort; }
     m := UpdateLocal(m, old_size + 29, tmp);
 
@@ -3503,7 +3505,7 @@ requires ExistsTxnSenderAccount(m, txn);
     call t10 := CopyOrMoveRef(t2);
 
     call tmp := ReadRef(t10);
-    assume IsValidInteger(tmp);
+    assume IsValidU64(tmp);
 
     m := UpdateLocal(m, old_size + 11, tmp);
 
@@ -3519,14 +3521,14 @@ requires ExistsTxnSenderAccount(m, txn);
     call t13 := CopyOrMoveRef(t2);
 
     call tmp := ReadRef(t13);
-    assume IsValidInteger(tmp);
+    assume IsValidU64(tmp);
 
     m := UpdateLocal(m, old_size + 14, tmp);
 
     call tmp := LdConst(1);
     m := UpdateLocal(m, old_size + 15, tmp);
 
-    call tmp := Add(GetLocal(m, old_size + 14), GetLocal(m, old_size + 15));
+    call tmp := AddU64(GetLocal(m, old_size + 14), GetLocal(m, old_size + 15));
     if (abort_flag) { goto Label_Abort; }
     m := UpdateLocal(m, old_size + 16, tmp);
 
@@ -3749,7 +3751,7 @@ requires ExistsTxnSenderAccount(m, txn);
     call t10 := CopyOrMoveRef(t2);
 
     call tmp := ReadRef(t10);
-    assume IsValidInteger(tmp);
+    assume IsValidU64(tmp);
 
     m := UpdateLocal(m, old_size + 11, tmp);
 
@@ -3762,14 +3764,14 @@ requires ExistsTxnSenderAccount(m, txn);
     call t13 := CopyOrMoveRef(t2);
 
     call tmp := ReadRef(t13);
-    assume IsValidInteger(tmp);
+    assume IsValidU64(tmp);
 
     m := UpdateLocal(m, old_size + 14, tmp);
 
     call tmp := LdConst(1);
     m := UpdateLocal(m, old_size + 15, tmp);
 
-    call tmp := Add(GetLocal(m, old_size + 14), GetLocal(m, old_size + 15));
+    call tmp := AddU64(GetLocal(m, old_size + 14), GetLocal(m, old_size + 15));
     if (abort_flag) { goto Label_Abort; }
     m := UpdateLocal(m, old_size + 16, tmp);
 
@@ -3909,7 +3911,7 @@ ensures old(b#Boolean(Boolean(!(b#Boolean(ExistsResource(m, LibraAccount_T_type_
 
     call t2 := LibraAccount_balance(GetLocal(m, old_size + 1));
     if (abort_flag) { goto Label_Abort; }
-    assume IsValidInteger(t2);
+    assume IsValidU64(t2);
 
     m := UpdateLocal(m, old_size + 2, t2);
 
