language/move-prover/bytecode-to-boogie/tests/goldenfiles/verify-addition.bpl
@@ -1,0 +1,267 @@
+
+
+// ** structs of module TestAddition
+
+
+
+// ** functions of module TestAddition
+
+procedure {:inline 1} TestAddition_overflow_u8_add_bad (x: Value, y: Value) returns (ret0: Value)
+requires ExistsTxnSenderAccount(m, txn);
+ensures old(!(b#Boolean(Boolean(false)))) ==> !abort_flag;
+ensures old(b#Boolean(Boolean(false))) ==> abort_flag;
+{
+    // declare local variables
+    var t2: Value; // IntegerType()
+    var t3: Value; // IntegerType()
+    var t4: Value; // IntegerType()
+
+    var tmp: Value;
+    var old_size: int;
+
+    var saved_m: Memory;
+    assume !abort_flag;
+    saved_m := m;
+
+    // assume arguments are of correct types
+    assume IsValidU8(x);
+    assume IsValidU8(y);
+
+    old_size := local_counter;
+    local_counter := local_counter + 5;
+    m := UpdateLocal(m, old_size + 0, x);
+    m := UpdateLocal(m, old_size + 1, y);
+
+    // bytecode translation starts here
+    call tmp := CopyOrMoveValue(GetLocal(m, old_size + 0));
+    m := UpdateLocal(m, old_size + 2, tmp);
+
+    call tmp := CopyOrMoveValue(GetLocal(m, old_size + 1));
+    m := UpdateLocal(m, old_size + 3, tmp);
+
+    call tmp := AddU8(GetLocal(m, old_size + 2), GetLocal(m, old_size + 3));
+    if (abort_flag) { goto Label_Abort; }
+    m := UpdateLocal(m, old_size + 4, tmp);
+
+    ret0 := GetLocal(m, old_size + 4);
+    return;
+
+Label_Abort:
+    abort_flag := true;
+    m := saved_m;
+    ret0 := DefaultValue;
+}
+
+procedure TestAddition_overflow_u8_add_bad_verify (x: Value, y: Value) returns (ret0: Value)
+{
+    assume ExistsTxnSenderAccount(m, txn);
+    call ret0 := TestAddition_overflow_u8_add_bad(x, y);
+}
+
+procedure {:inline 1} TestAddition_overflow_u8_add_ok (x: Value, y: Value) returns (ret0: Value)
+requires ExistsTxnSenderAccount(m, txn);
+ensures old(!(b#Boolean(Boolean(i#Integer(Integer(i#Integer(x) + i#Integer(y))) > i#Integer(Integer(255)))))) ==> !abort_flag;
+ensures old(b#Boolean(Boolean(i#Integer(Integer(i#Integer(x) + i#Integer(y))) > i#Integer(Integer(255))))) ==> abort_flag;
+{
+    // declare local variables
+    var t2: Value; // IntegerType()
+    var t3: Value; // IntegerType()
+    var t4: Value; // IntegerType()
+
+    var tmp: Value;
+    var old_size: int;
+
+    var saved_m: Memory;
+    assume !abort_flag;
+    saved_m := m;
+
+    // assume arguments are of correct types
+    assume IsValidU8(x);
+    assume IsValidU8(y);
+
+    old_size := local_counter;
+    local_counter := local_counter + 5;
+    m := UpdateLocal(m, old_size + 0, x);
+    m := UpdateLocal(m, old_size + 1, y);
+
+    // bytecode translation starts here
+    call tmp := CopyOrMoveValue(GetLocal(m, old_size + 0));
+    m := UpdateLocal(m, old_size + 2, tmp);
+
+    call tmp := CopyOrMoveValue(GetLocal(m, old_size + 1));
+    m := UpdateLocal(m, old_size + 3, tmp);
+
+    call tmp := AddU8(GetLocal(m, old_size + 2), GetLocal(m, old_size + 3));
+    if (abort_flag) { goto Label_Abort; }
+    m := UpdateLocal(m, old_size + 4, tmp);
+
+    ret0 := GetLocal(m, old_size + 4);
+    return;
+
+Label_Abort:
+    abort_flag := true;
+    m := saved_m;
+    ret0 := DefaultValue;
+}
+
+procedure TestAddition_overflow_u8_add_ok_verify (x: Value, y: Value) returns (ret0: Value)
+{
+    assume ExistsTxnSenderAccount(m, txn);
+    call ret0 := TestAddition_overflow_u8_add_ok(x, y);
+}
+
+procedure {:inline 1} TestAddition_overflow_u64_add_bad (x: Value, y: Value) returns (ret0: Value)
+requires ExistsTxnSenderAccount(m, txn);
+ensures old(!(b#Boolean(Boolean(false)))) ==> !abort_flag;
+ensures old(b#Boolean(Boolean(false))) ==> abort_flag;
+{
+    // declare local variables
+    var t2: Value; // IntegerType()
+    var t3: Value; // IntegerType()
+    var t4: Value; // IntegerType()
+
+    var tmp: Value;
+    var old_size: int;
+
+    var saved_m: Memory;
+    assume !abort_flag;
+    saved_m := m;
+
+    // assume arguments are of correct types
+    assume IsValidU64(x);
+    assume IsValidU64(y);
+
+    old_size := local_counter;
+    local_counter := local_counter + 5;
+    m := UpdateLocal(m, old_size + 0, x);
+    m := UpdateLocal(m, old_size + 1, y);
+
+    // bytecode translation starts here
+    call tmp := CopyOrMoveValue(GetLocal(m, old_size + 0));
+    m := UpdateLocal(m, old_size + 2, tmp);
+
+    call tmp := CopyOrMoveValue(GetLocal(m, old_size + 1));
+    m := UpdateLocal(m, old_size + 3, tmp);
+
+    call tmp := AddU64(GetLocal(m, old_size + 2), GetLocal(m, old_size + 3));
+    if (abort_flag) { goto Label_Abort; }
+    m := UpdateLocal(m, old_size + 4, tmp);
+
+    ret0 := GetLocal(m, old_size + 4);
+    return;
+
+Label_Abort:
+    abort_flag := true;
+    m := saved_m;
+    ret0 := DefaultValue;
+}
+
+procedure TestAddition_overflow_u64_add_bad_verify (x: Value, y: Value) returns (ret0: Value)
+{
+    assume ExistsTxnSenderAccount(m, txn);
+    call ret0 := TestAddition_overflow_u64_add_bad(x, y);
+}
+
+procedure {:inline 1} TestAddition_overflow_u64_add_ok (x: Value, y: Value) returns (ret0: Value)
+requires ExistsTxnSenderAccount(m, txn);
+ensures old(!(b#Boolean(Boolean(i#Integer(Integer(i#Integer(x) + i#Integer(y))) > i#Integer(Integer(9223372036854775807)))))) ==> !abort_flag;
+ensures old(b#Boolean(Boolean(i#Integer(Integer(i#Integer(x) + i#Integer(y))) > i#Integer(Integer(9223372036854775807))))) ==> abort_flag;
+{
+    // declare local variables
+    var t2: Value; // IntegerType()
+    var t3: Value; // IntegerType()
+    var t4: Value; // IntegerType()
+
+    var tmp: Value;
+    var old_size: int;
+
+    var saved_m: Memory;
+    assume !abort_flag;
+    saved_m := m;
+
+    // assume arguments are of correct types
+    assume IsValidU64(x);
+    assume IsValidU64(y);
+
+    old_size := local_counter;
+    local_counter := local_counter + 5;
+    m := UpdateLocal(m, old_size + 0, x);
+    m := UpdateLocal(m, old_size + 1, y);
+
+    // bytecode translation starts here
+    call tmp := CopyOrMoveValue(GetLocal(m, old_size + 0));
+    m := UpdateLocal(m, old_size + 2, tmp);
+
+    call tmp := CopyOrMoveValue(GetLocal(m, old_size + 1));
+    m := UpdateLocal(m, old_size + 3, tmp);
+
+    call tmp := AddU64(GetLocal(m, old_size + 2), GetLocal(m, old_size + 3));
+    if (abort_flag) { goto Label_Abort; }
+    m := UpdateLocal(m, old_size + 4, tmp);
+
+    ret0 := GetLocal(m, old_size + 4);
+    return;
+
+Label_Abort:
+    abort_flag := true;
+    m := saved_m;
+    ret0 := DefaultValue;
+}
+
+procedure TestAddition_overflow_u64_add_ok_verify (x: Value, y: Value) returns (ret0: Value)
+{
+    assume ExistsTxnSenderAccount(m, txn);
+    call ret0 := TestAddition_overflow_u64_add_ok(x, y);
+}
+
+procedure {:inline 1} TestAddition_overflow_u128_add_bad (x: Value, y: Value) returns (ret0: Value)
+requires ExistsTxnSenderAccount(m, txn);
+ensures old(!(b#Boolean(Boolean(false)))) ==> !abort_flag;
+ensures old(b#Boolean(Boolean(false))) ==> abort_flag;
+{
+    // declare local variables
+    var t2: Value; // IntegerType()
+    var t3: Value; // IntegerType()
+    var t4: Value; // IntegerType()
+
+    var tmp: Value;
+    var old_size: int;
+
+    var saved_m: Memory;
+    assume !abort_flag;
+    saved_m := m;
+
+    // assume arguments are of correct types
+    assume IsValidU128(x);
+    assume IsValidU128(y);
+
+    old_size := local_counter;
+    local_counter := local_counter + 5;
+    m := UpdateLocal(m, old_size + 0, x);
+    m := UpdateLocal(m, old_size + 1, y);
+
+    // bytecode translation starts here
+    call tmp := CopyOrMoveValue(GetLocal(m, old_size + 0));
+    m := UpdateLocal(m, old_size + 2, tmp);
+
+    call tmp := CopyOrMoveValue(GetLocal(m, old_size + 1));
+    m := UpdateLocal(m, old_size + 3, tmp);
+
+    call tmp := AddU128(GetLocal(m, old_size + 2), GetLocal(m, old_size + 3));
+    if (abort_flag) { goto Label_Abort; }
+    m := UpdateLocal(m, old_size + 4, tmp);
+
+    ret0 := GetLocal(m, old_size + 4);
+    return;
+
+Label_Abort:
+    abort_flag := true;
+    m := saved_m;
+    ret0 := DefaultValue;
+}
+
+procedure TestAddition_overflow_u128_add_bad_verify (x: Value, y: Value) returns (ret0: Value)
+{
+    assume ExistsTxnSenderAccount(m, txn);
+    call ret0 := TestAddition_overflow_u128_add_bad(x, y);
+}
